protocols/SafeProtocol.v
@@ -1,0 +1,120 @@
+(* DISTRIBUTION STATEMENT A. Approved for public release. Distribution is unlimited.
+ *
+ * This material is based upon work supported by the Department of the Air Force under Air Force 
+ * Contract No. FA8702-15-D-0001. Any opinions, findings, conclusions or recommendations expressed 
+ * in this material are those of the author(s) and do not necessarily reflect the views of the 
+ * Department of the Air Force.
+ * 
+ * © 2019 Massachusetts Institute of Technology.
+ * 
+ * MIT Proprietary, Subject to FAR52.227-11 Patent Rights - Ownership by the contractor (May 2014)
+ * 
+ * The software/firmware is provided to you on an As-Is basis
+ * 
+ * Delivered to the U.S. Government with Unlimited Rights, as defined in DFARS Part 252.227-7013
+ * or 7014 (Feb 2014). Notwithstanding any copyright notice, U.S. Government rights in this work are
+ * defined by DFARS 252.227-7013 or DFARS 252.227-7014 as detailed above. Use of this work other than
+ * as specifically authorized by the U.S. Government may violate any copyrights that exist in this work. *)
+
+From Coq Require Import
+     List.
+
+Require Import
+        MyPrelude
+        Maps
+        Messages
+        Tactics
+        Simulation
+        RealWorld
+        AdversarySafety.
+
+Require IdealWorld.
+Import RealWorld.RealWorldNotations.
+
+Set Implicit Arguments.
+
+Definition adversary_is_lame {B : type} (b : << Base B >>) (adv : user_data B) : Prop :=
+    adv.(key_heap) = $0
+  /\ adv.(msg_heap) = []
+  /\ adv.(c_heap) = []
+  /\ lameAdv b adv.
+
+Definition universe_starts_sane {A B : type} (b : << Base B >>) (U : universe A B) : Prop :=
+  let honestk := findUserKeys U.(users)
+  in  (forall u_id u, U.(users) $? u_id = Some u -> u.(RealWorld.msg_heap) = [])
+      /\ ciphers_honestly_signed honestk U.(RealWorld.all_ciphers)
+      /\ keys_honest honestk U.(RealWorld.all_keys)
+      /\ adversary_is_lame b U.(adversary).
+
+(* 
+ * Our definition of a Safe Protocol.  For now, we assume a pretty boring initial
+ * adversary state.  The constraints could be relaxed a bit, but it is unclear that
+ * there is really any purpose in doing so.
+ *)
+Module Type SafeProtocol.
+
+  Parameter A B : type.
+  Parameter U__i : IdealWorld.universe A.
+  Parameter U__r : universe A B.
+  Parameter b : << Base B >>.
+  Parameter R : simpl_universe A -> IdealWorld.universe A -> Prop.
+
+  Axiom U_good : universe_starts_sane b U__r.
+
+  Axiom R_silent_simulates : simulates_silent_step (lameAdv b) R.
+  Axiom R_loud_simulates : simulates_labeled_step (lameAdv b) R.
+  Axiom R_honest_actions_safe : honest_actions_safe B R.
+  Axiom universe_starts_safe : R (peel_adv U__r) U__i /\ universe_ok U__r /\ adv_universe_ok U__r.
+
+End SafeProtocol.
+
+(*
+ * A Functor which lifts any 'SafeProtocol' into the state we really want,
+ * namely a universe where there is an adversary executing arbitrary code.
+ * This lifting is basically provided by the top level proofs of
+ * AdversarySafety.
+ *)
+
+Module AdversarySafeProtocol ( Proto : SafeProtocol ).
+  Import Proto.
+
+  Hint Resolve
+       R_silent_simulates
+       R_loud_simulates
+       R_honest_actions_safe.
+
+  Lemma proto_lamely_refines :
+    refines (lameAdv b) U__r U__i.
+  Proof.
+    exists R; unfold simulates.
+    pose proof universe_starts_safe.
+    intuition eauto.
+  Qed.
+
+  Hint Resolve proto_lamely_refines.
+
+  Lemma proto_starts_ok : universe_starts_ok U__r.
+  Proof.
+    pose proof universe_starts_safe.
+    pose proof U_good.
+    unfold universe_starts_ok; intros.
+    unfold universe_ok, adv_universe_ok, universe_starts_sane in *; split_ands.
+    intuition eauto.
+  Qed.
+
+  Hint Resolve proto_starts_ok.
+
+  Theorem protocol_with_adversary_could_generate_spec :
+    forall U__ra advcode acts__r,
+      U__ra = add_adversary U__r advcode
+      -> rCouldGenerate U__ra acts__r
+      -> exists acts__i,
+          iCouldGenerate U__i acts__i
+          /\ traceMatches acts__r acts__i.
+  Proof.
+    intros.
+    pose proof U_good as L; unfold universe_starts_sane, adversary_is_lame in L; split_ands.
+    eapply refines_could_generate; eauto.
+  Qed.
+  
+End AdversarySafeProtocol.
